ssreflect first try

RE.v
@@ -1,10 +1,9 @@
+Require Import ssreflect ssrbool eqtype ssrnat.
+
 Require Import Coq.Lists.List.
-Require Import finite_type.
-Require Import props.
 
 Section RE.
-Variable A:Type.
-Variable eqA: forall a b : A, {a=b} + {~a=b}.
+Variable A:eqType.
 
 Definition word := list A.
 
@@ -21,16 +20,16 @@ match r with
 | Null => false
 | Empty => true
 | Char _ => false
-| Plus r s => orb (has_empty r) (has_empty s)
+| Plus r s => (has_empty r) || (has_empty s)
 | Star r => true
-| Conc r s => andb (has_empty r) (has_empty s)
+| Conc r s => (has_empty r) && (has_empty s)
 end.
 
 Fixpoint der r a :=
 match r with
 | Null => Null
 | Empty => Null
-| Char a' => if eqA a a' then Empty else Null
+| Char a' => if a==a' then Empty else Null
 | Star r => Conc (der r a) (Star r)
 | Plus r s => Plus (der r a) (der s a)
 | Conc r s => if has_empty r then Plus (Conc (der r a) s) (der s a) else Conc (der r a) s
@@ -48,55 +47,52 @@ match w with
 | cons a w' =>  mem_der (der r a) w'
 end.
 
-Lemma mem_der_Null w : mem_der Null w = true -> False.
-Proof. induction w. discriminate. eauto. Qed.
+Lemma mem_der_Null w : mem_der Null w -> False.
+Proof. induction w => //. Qed.
 
-Lemma mem_der_Empty w : mem_der Empty w = true -> w = nil.
-Proof. induction w. reflexivity. simpl. intros B. destruct (mem_der_Null _ B). Qed.
+Lemma mem_der_Empty w : mem_der Empty w -> w = nil.
+Proof. induction w => //. move => B. destruct (mem_der_Null _ B). Qed.
 
 Lemma mem_der_Char a w : mem_der (Char a) w = true -> w = cons a nil.
 Proof.
-induction w. discriminate.
-  simpl. intros B. destruct (eqA a0 a). 
-    assert (w = nil) by (eauto using mem_der_Empty). subst. reflexivity.
-    elimtype False; eauto using mem_der_Null.
+induction w => //=.
+case_eq (a0 == a); move/eqP.
+  by move => -> /mem_der_Empty -> //.
+by move => F /mem_der_Null => //.
 Qed.
 
-Lemma mem_der_Plus r1 r2 w: mem_der (Plus r1 r2) w = true -> {mem_der r1 w=true}+{mem_der r2 w=true}.
+Lemma mem_der_Plus r1 r2 w: mem_der (Plus r1 r2) w -> {mem_der r1 w}+{mem_der r2 w}.
 Proof.
-revert r1 r2 w. fix f 3. destruct w as [|a w]; simpl. 
-  destruct (has_empty r1), (has_empty r2); eauto.
-  intros B. destruct (f (der r1 a) (der r2 a) w); eauto. 
+move: r1 r2 w. fix f 3. move=> r1 r2. case; simpl. 
+  case_eq (has_empty r1); case_eq (has_empty r2); auto.
+  move=> a l B. case: (f (der r1 a) (der r2 a) l); auto. 
 Qed.
 
-Lemma mem_der_Conc_Null r w: mem_der (Conc Null r) w = true -> False.
-Proof.
-induction w. discriminate.
-simpl. eauto.
-Qed.
+Lemma mem_der_Conc_Null r w: mem_der (Conc Null r) w -> False.
+Proof. induction w => //=. Qed.
 
 Lemma der_not_Char r a c: der r a <> Char c.
 Proof.
-induction r; simpl; try discriminate. destruct (eqA a c0); discriminate.
-destruct (has_empty r1); discriminate.
+induction r; simpl; try discriminate. case: (a == c0); discriminate.
+case: (has_empty r1); discriminate.
 Qed.
 
-Lemma mem_der_Plus' r s w : mem_der r w = true \/ mem_der s w = true -> mem_der (Plus r s) w = true.
+Lemma mem_der_Plus' r s w : mem_der r w \/ mem_der s w -> mem_der (Plus r s) w.
 Proof.
-revert r s. induction w; simpl; intros r s.
-  intros [B|B]; rewrite B; try reflexivity. destruct (has_empty r); reflexivity.
-  eauto. 
+move: r s. induction w => //=; move=> r s.
+  move => [] -> //; case: (has_empty r) => //.
+auto. 
 Qed.
 
-Lemma mem_der_Conc r s w1 w2 : mem_der r w1 = true ->  mem_der s w2 = true ->
-mem_der (Conc r s) (w1 ++ w2) = true.
+Lemma mem_der_Conc r s w1 w2 : mem_der r w1 ->  mem_der s w2 ->
+mem_der (Conc r s) (w1 ++ w2).
 Proof.
-revert r s w2. induction w1; simpl; intros r s w2 B C.
-revert r s B C. induction w2; simpl; intros r s B C. rewrite B,C. reflexivity.
-simpl in *. rewrite B. apply mem_der_Plus'. eauto.
-case_eq (has_empty r); simpl; intros D.
-apply mem_der_Plus'. left. apply IHw1; assumption.
-apply IHw1; assumption.
+move: r s w2. induction w1 => r s w2 B C /=.
+  move: r s B C. induction w2 => /= r s -> //. 
+  move => C. apply/mem_der_Plus'. by auto. 
+case: (has_empty r) => /=.
+  apply/mem_der_Plus'. left. by apply/IHw1 => //.
+by apply/IHw1 => //.
 Qed.
 
 
@@ -112,109 +108,125 @@ Inductive lang : re -> word -> Prop :=
 .
 
 Lemma lang_nil_w r w : lang r (nil ++ w) -> lang r w.
-Proof. simpl. auto. Qed.
+Proof. by []. Qed.
 
 Lemma append_nil w : (w ++ @nil A) = w.
-Proof. induction w. eauto. simpl. rewrite IHw. reflexivity. Qed.
+Proof. induction w => //=. by rewrite IHw => //. Qed.
 
 Lemma lang_w_nil r w : lang r (w ++ nil) -> lang r w. 
-Proof. rewrite append_nil; eauto. Qed.
+Proof. by rewrite append_nil => //. Qed.
 
-Lemma lang_empty_nil r : has_empty r = true -> lang r nil.
-Proof. induction r; try (discriminate || now constructor); simpl; intros H; 
-destruct (has_empty r1), (has_empty r2); eauto using lang, lang_w_nil.
+Lemma lang_w_nil' r w : lang r (nil ++ w) -> lang r w. 
+Proof. by simpl => //. Qed.
+
+Lemma lang_empty_nil r : has_empty r -> lang r nil.
+Proof. induction r => /=; try (discriminate || now constructor); move => H;
+move: IHr1 IHr2 H; case: (has_empty r1); case: (has_empty r2); 
+by eauto using lang_nil_w, lang.
 Qed.
 
 Lemma append_backwards (a:A) w1 w2: cons a (w1 ++ w2) = ((cons a w1) ++ w2).
-Proof. reflexivity. Qed.
+Proof. by []. Qed.
 
 Lemma lang_der r a w : lang (der r a) w -> lang r (cons a w).
 Proof.
-revert a w. induction r; intros a w; simpl; intros B; 
-  try now (inversion B; eauto using lang).
+move: a w. induction r => a w /=;
+  try now (move => B; inversion B; eauto using lang).
 (* lang (Char c) (a::w) *) 
-  destruct (eqA a c); inversion B; subst; constructor.
+  case_eq (a == c); move/eqP.
+    move => -> B. inversion B. constructor.
+  move => F B. inversion B.
 (* lang (Conc r1 r2) (a::w) *) 
-  case_eq (has_empty r1); intros C; rewrite C in *.
-(* has_empty r1 = true *)
+  case_eq (has_empty r1) => /= C B.
+  (* has_empty r1 = true *)
     inversion B; subst.
-      inversion H2. subst. rewrite (append_backwards a w1 w2). constructor; eauto. 
-      apply lang_nil_w. constructor. eauto using lang_empty_nil. eauto.
-(* has_empty r1 = false *)
-  inversion B; subst. rewrite (append_backwards a w1 w2). eauto using lang.
+      inversion H2; subst. rewrite (append_backwards a w1 w2). constructor; eauto. 
+      apply lang_w_nil'. constructor. 
+        exact: lang_empty_nil. 
+      exact: IHr2.
+  (* has_empty r1 = false *)
+    inversion B; subst. rewrite (append_backwards a w1 w2). eauto using lang.
 (* lang (Star r) (a::w) *)
-  inversion B; subst. constructor. rewrite (append_backwards). apply langConc; eauto.
+  move => B; inversion B; subst. constructor. rewrite (append_backwards). apply/langConc; auto.
 Qed. 
 
 Lemma mem_der_lang_agree r w : mem_der r w = true <-> lang r w.
 Proof. split.
-revert r. induction w; intros r; simpl. apply lang_empty_nil.
-remember (der r a) as s. induction s; intros B. 
+move: r. induction w => r /=. 
+exact: lang_empty_nil.
+
+remember (der r a) as s. induction s.
 (* der r a = Null *) 
-  destruct (mem_der_Null _ B).
+  by move => /mem_der_Null.
 
 (* der r a = Empty *) 
-  rewrite (mem_der_Empty _ B). destruct r; try discriminate.
+  move => /mem_der_Empty. destruct r; try by [].
   (* r = Char c *)
-    simpl in Heqs. destruct (eqA a c) as [C|C]. 
-      rewrite C in *. constructor.
-      discriminate.
+    move : Heqs => /=. case_eq (a==c). 
+      move/eqP => -> _ ->. by constructor.
+    by [].
+  
   (* r = Conc r1 r2 *)
-    simpl in Heqs. destruct (has_empty r1); discriminate.
+    move: Heqs => /=. case: (has_empty r1); discriminate.
 
 (* der r a = Char c *)
-  symmetry in Heqs.
-  destruct (der_not_Char _ _ _ Heqs).
+  have: (der r a = Char c). 
+    by symmetry in Heqs.
+  by move/der_not_Char.
 
 (* der r a = Conc s1 s2 *)
-  rewrite Heqs in B. apply lang_der. apply IHw. assumption.
-  destruct r; try discriminate; simpl in Heqs.
+  rewrite Heqs. move/IHw. 
+  destruct r; move: Heqs => //=.
   (* r = Char c *)
-    destruct (eqA a c); discriminate.
+    by case_eq (a == c).
   (* r = Conc r1 r2 *)
-    case_eq (has_empty r1); intros E; rewrite E in Heqs. inversion Heqs. subst.
-    destruct (mem_der_Plus _ _ _ B) as [C|C].
-      assert (lang (Conc (der r1 a) r2) w). eauto.
-      inversion H. subst. rewrite (append_backwards a w1 w2). 
-        constructor. apply lang_der. assumption. assumption.
-      apply (langConc _ _ (nil)). apply lang_empty_nil. assumption.
-      assert (lang r2 (cons a w)). apply lang_der. apply IHw. assumption.
-      assumption.
-      discriminate.
+    case_eq (has_empty r1) => E Heqs B; inversion Heqs. inversion B; subst.
+      rewrite append_backwards. constructor. by apply/lang_der. 
+    by [].
+  (* r = Star r *)
+    move => Heqs B. inversion Heqs; inversion B; subst.
+    rewrite append_backwards. constructor. constructor; [exact: lang_der | by [] ].
 
 (* der r a = Plus r1 r2 *)
-  inversion Heqs. subst.
-  destruct (mem_der_Plus _ _ _ B) as [C|C].
-  apply langPlusL. apply lang_der. apply IHw. assumption.
-  apply langPlusR. apply lang_der. apply IHw. assumption.
+  destruct r; move: Heqs => //=.
+  (* r = Char c *)
+    by case_eq (a == c).
+  (* r = Conc r1 r2 *)
+    case_eq (has_empty r1) => E Heqs. inversion Heqs; subst.
+    (* has_empty r1 = true *)
+      move/mem_der_Plus => []. move/IHw => B. inversion B. subst.
+      rewrite append_backwards. constructor; [exact: lang_der | by [] ].
+    move => B. apply/lang_w_nil'. move/IHw/lang_der : B. move/lang_empty_nil: E.
+    exact: langConc.
+    (* has_empty r1 = true *)
+    inversion Heqs.
+  (* r = Plus r1 r2 *)
+  move => B. inversion B; subst. 
+  move /mem_der_Plus => [] /IHw /lang_der; [exact: langPlusL | exact: langPlusR].
 
 (* der r a = Star s *)
-  destruct r; try discriminate; simpl in Heqs.
+  destruct r; try discriminate; move: Heqs => //=.
   (* r = Char c *)
-    destruct (eqA a c); discriminate Heqs.
+    by case_eq (a == c).
   (* r = Star s *)
-    destruct (has_empty r1); discriminate Heqs.
+    by case: (has_empty r1).
 
 
 (* <- *)
-intros B. induction B.
-(* mem_der Empty nil *)
-  reflexivity.
+move=>B. induction B => //=.
 (* mem_der (Char a) (a::nil) *)
-  simpl. destruct (eqA a a). reflexivity. assert False as []. apply n. reflexivity.
-(* mem_der (Plus r s) w *)
-  apply mem_der_Plus'. eauto.
-  apply mem_der_Plus'. eauto.
+  simpl. by rewrite eq_refl.
+(* mem_der (Plus r s) w *) 
+  apply mem_der_Plus'. by left.
+  apply mem_der_Plus'. by right.
 (* mem_der (Conc r s) (w1 ++ w2) *)
-  apply mem_der_Conc; assumption.
-(* mem_der (Star r) nil *)
-  reflexivity.
+  by apply mem_der_Conc.
 (* mem_der (Star r) w *)
-  induction w. reflexivity.
-  inversion B. subst. rewrite H1. simpl in *.
-  case_eq (has_empty r); intros C; rewrite C in IHB.
-    destruct (mem_der_Plus _ _ _ IHB) as [E|E]; assumption.
-    assumption.
+  induction w => //=. 
+  inversion B. subst.
+  move: IHB => /=. case: (has_empty r).
+    by move/mem_der_Plus => [].
+  by [].
 Qed.
 
 
